Completed new static analysis.

gen/su/nsk/iae/reflex/antlr/ReflexBaseVisitor.java
@@ -3,6 +3,8 @@ package su.nsk.iae.reflex.antlr;
 import org.antlr.v4.runtime.tree.AbstractParseTreeVisitor;
 import su.nsk.iae.reflex.antlr.ReflexVisitor;
 import su.nsk.iae.reflex.antlr.ReflexParser;
+
+
 /**
  * This class provides an empty implementation of {@link ReflexVisitor},
  * which can be extended to create a visitor which only needs to handle a subset
