src/main/java/su/nsk/iae/reflex/staticAnalysis/RuleChecker.java
@@ -1,2 +1,99 @@
-package su.nsk.iae.reflex.staticAnalysis;public class RuleChecker {
+package su.nsk.iae.reflex.staticAnalysis;
+
+import su.nsk.iae.reflex.antlr.ReflexParser;
+import su.nsk.iae.reflex.staticAnalysis.attributes.*;
+import su.nsk.iae.reflex.vcg.ProgramMetaData;
+
+import java.util.Deque;
+import java.util.List;
+import java.util.Stack;
+
+public class RuleChecker {
+    ProgramMetaData metaData;
+    public RuleChecker(ProgramMetaData metaData){
+        this.metaData = metaData;
+    }
+
+    public boolean checkTimeout(Deque<IAttributed> path){
+        for (IAttributed attr: path){
+            switch (attr.getContextType()){
+                case Process:{
+                    return true;
+                }
+                case IfElse:{
+                    IfElseAttributes newAttr = (IfElseAttributes) attr;
+                    if(newAttr.isReset()) return false;
+                }
+                case SwitchCase:{
+                    SwitchCaseAttributes newAttr = (SwitchCaseAttributes) attr;
+                    if(newAttr.isReset()) return false;
+                }
+            }
+        }
+        return true;
+    }
+
+    public boolean checkRules(Deque<IAttributed> path, IAttributed attr){
+        switch (attr.getContextType()){
+            case Process: {
+                for (IAttributed pattr: path) {
+                    if (!checkRulesProcessAttributes(pattr,(ProcessAttributes) attr)) return false;
+                }
+                return true;
+            }
+            default: return true;
+        }
+    }
+
+    private boolean checkRulesProcessAttributes(IAttributed attr1, ProcessAttributes attr2){
+        if(!attr2.isReachE() && attr2.getState().equals("error"))return false;
+        if(!attr2.isReachS() && !attr2.isStartS() && attr2.getState().equals("break")) return false;
+        switch (attr1.getContextType()){
+            case IfElse :{
+                IfElseAttributes newAttr1 = (IfElseAttributes) attr1;
+                ChangeType t = newAttr1.getProcChange().get(attr2.getAttributedContext());
+                if (t==null) return true;
+                return switch (t) {
+                    case Start -> {
+                        ReflexParser.ProcessContext p = (ReflexParser.ProcessContext) attr2.getAttributedContext();
+                        yield metaData.isFirstState(p.name.getText(), attr2.getState());
+                    }
+                    case Stop -> attr2.getState().equals("break");
+                    case Error -> attr2.getState().equals("error");
+                };
+            }
+            case SwitchCase:{
+                SwitchCaseAttributes newAttr1 = (SwitchCaseAttributes) attr1;
+                ChangeType t = newAttr1.getProcChange().get(attr2.getAttributedContext());
+                if (t==null) return true;
+                return switch (t) {
+                    case Start -> {
+                        ReflexParser.ProcessContext p = (ReflexParser.ProcessContext) attr2.getAttributedContext();
+                        yield metaData.isFirstState(p.name.getText(), attr2.getState());
+                    }
+                    case Stop -> attr2.getState().equals("break");
+                    case Error -> attr2.getState().equals("error");
+                };
+            }
+            case State:{
+                StateAttributes newAttr1 = (StateAttributes) attr1;
+                ChangeType t = newAttr1.getProcChange().get(attr2.getAttributedContext());
+                if (t==null) return true;
+                return switch (t) {
+                    case Start -> {
+                        ReflexParser.ProcessContext p = (ReflexParser.ProcessContext) attr2.getAttributedContext();
+                        yield metaData.isFirstState(p.name.getText(), attr2.getState());
+                    }
+                    case Stop -> attr2.getState().equals("break");
+                    case Error -> attr2.getState().equals("error");
+                };
+            }
+            case Process:{
+                return true;
+            }
+
+        }
+        return true;
+    }
+
 }
