src/main/java/su/nsk/iae/reflex/staticAnalysis/attributes/AttributeCollector.java
@@ -1,2 +1,17 @@
-package su.nsk.iae.reflex.staticAnalysis.attributes;public class AttributeCollector {
+package su.nsk.iae.reflex.staticAnalysis.attributes;
+
+import org.antlr.v4.runtime.ParserRuleContext;
+
+import java.util.HashMap;
+
+public class AttributeCollector {
+    HashMap<ParserRuleContext,IAttributed> attributeMap = new HashMap<>();;
+
+    public void addAttributes(ParserRuleContext context,IAttributed attributed){
+        attributeMap.put(context,attributed);
+    }
+
+    public IAttributed getAttributes(ParserRuleContext context){
+        return attributeMap.get(context);
+    }
 }
