src/main/java/su/nsk/iae/reflex/staticAnalysis/attributes/AttributedContextType.java
@@ -1,4 +1,4 @@
-package su.nsk.iae.reflex.staticAnalysis;
+package su.nsk.iae.reflex.staticAnalysis.attributes;
 
 public enum AttributedContextType {
     Process,State,IfElse,SwitchCase
