src/main/java/su/nsk/iae/reflex/staticAnalysis/attributes/ChangeType.java
@@ -1,2 +1,5 @@
-package su.nsk.iae.reflex.staticAnalysis.attributes;public enum ChangeType {
+package su.nsk.iae.reflex.staticAnalysis.attributes;
+
+public enum ChangeType {
+    Start,Stop,Error
 }
