src/main/java/su/nsk/iae/reflex/staticAnalysis/attributes/ProcessActivity.java
@@ -1,4 +1,4 @@
-package su.nsk.iae.reflex.staticAnalysis;
+package su.nsk.iae.reflex.staticAnalysis.attributes;
 
 public enum ProcessActivity {
     Active,Inactive,Stop,Error
