src/main/java/su/nsk/iae/reflex/staticAnalysis/attributes/ProcessAttributes.java
@@ -1,11 +1,67 @@
-package su.nsk.iae.reflex.staticAnalysis;
+package su.nsk.iae.reflex.staticAnalysis.attributes;
 
 import org.antlr.v4.runtime.ParserRuleContext;
 import su.nsk.iae.reflex.antlr.ReflexParser;
 
-public class ProcessAttributes implements Attributed{
+
+import java.util.HashMap;
+
+public class ProcessAttributes implements IAttributed {
 
     ParserRuleContext attributedContext;
-    ReflexParser.StateContext state;
+    String state;
 
+    boolean reachE = false;
+    boolean reachS = false;
+    boolean startS = true;
+
+    public ProcessAttributes(ReflexParser.ProcessContext attributedContext){
+        this.attributedContext = attributedContext;
+    }
+
+    public void setAttributedContext(ParserRuleContext attributedContext) {
+        this.attributedContext = attributedContext;
+    }
+
+    public String getState() {
+        return state;
+    }
+
+    public void setState(String state) {
+        this.state = state;
+    }
+
+    @Override
+    public ParserRuleContext getAttributedContext() {
+        return attributedContext;
+    }
+
+    @Override
+    public AttributedContextType getContextType() {
+        return AttributedContextType.Process;
+    }
+
+    public boolean isReachE() {
+        return reachE;
+    }
+
+    public void setReachE(boolean reachE) {
+        this.reachE = reachE;
+    }
+
+    public boolean isReachS() {
+        return reachS;
+    }
+
+    public void setReachS(boolean reachS) {
+        this.reachS = reachS;
+    }
+
+    public boolean isStartS() {
+        return startS;
+    }
+
+    public void setStartS(boolean startS) {
+        this.startS = startS;
+    }
 }
