src/main/java/su/nsk/iae/reflex/staticAnalysis/attributes/StateAttributes.java
@@ -1,22 +1,89 @@
-package su.nsk.iae.reflex.staticAnalysis;
+package su.nsk.iae.reflex.staticAnalysis.attributes;
 
 import org.antlr.v4.runtime.ParserRuleContext;
 import org.antlr.v4.runtime.misc.Pair;
 import su.nsk.iae.reflex.antlr.ReflexParser;
 
+import java.util.HashMap;
 import java.util.Vector;
 
-public class StateAttributes implements Attributed{
+public class StateAttributes implements IAttributed {
     ParserRuleContext attributedContext;
     ReflexParser.ProcessContext rootProcess;
-    boolean reachE = false;
-    boolean reachS = false;
-    boolean startS = true;
 
-    Vector<ReflexParser.ProcessContext> start = null;
-    Vector<ReflexParser.ProcessContext> stop = null;
-    Vector<ReflexParser.ProcessContext> error = null;
-    Vector<Pair<ReflexParser.ProcessContext,ProcessActivity>> activity= null;
+    HashMap<ReflexParser.ProcessContext,ChangeType> procChange = new HashMap<>();
     boolean reset = false;
     boolean stateChange = false;
+
+    ReflexParser.StateContext setState = null;
+
+    public StateAttributes(ReflexParser.ProcessContext process, ReflexParser.StateContext attributedContext){
+        rootProcess = process;
+        this.attributedContext = attributedContext;
+    }
+
+    public void setAttributedContext(ParserRuleContext attributedContext) {
+        this.attributedContext = attributedContext;
+    }
+
+    public ReflexParser.ProcessContext getRootProcess() {
+        return rootProcess;
+    }
+
+    public void setRootProcess(ReflexParser.ProcessContext rootProcess) {
+        this.rootProcess = rootProcess;
+    }
+
+
+    public boolean isReset() {
+        return reset;
+    }
+
+    public void setReset(boolean reset) {
+        this.reset = reset;
+    }
+
+    public boolean isStateChange() {
+        return stateChange;
+    }
+
+    public void setStateChange(boolean stateChange) {
+        this.stateChange = stateChange;
+    }
+
+    public ReflexParser.StateContext getSetState() {
+        return setState;
+    }
+
+    public void setSetState(ReflexParser.StateContext setState) {
+        this.setState = setState;
+    }
+
+    @Override
+    public ParserRuleContext getAttributedContext() {
+        return attributedContext;
+    }
+
+    public HashMap<ReflexParser.ProcessContext, ChangeType> getProcChange() {
+        return procChange;
+    }
+
+    public void setProcChange(HashMap<ReflexParser.ProcessContext, ChangeType> procChange) {
+        this.procChange = procChange;
+    }
+
+    public void addReset(boolean reset){
+        this.reset = this.reset || reset;
+    }
+
+    public void addProcessChange(ReflexParser.ProcessContext ctx, ChangeType type){
+        this.procChange.put(ctx,type);
+    }
+    public void addProcessChange(HashMap<ReflexParser.ProcessContext, ChangeType> other){
+        this.procChange.putAll(other);
+    }
+    @Override
+    public AttributedContextType getContextType() {
+        return AttributedContextType.State;
+    }
 }
