src/main/java/su/nsk/iae/reflex/staticAnalysis/attributes/SwitchCaseCore.java
@@ -1,2 +1,72 @@
-package su.nsk.iae.reflex.staticAnalysis.attributes;public class SwitchCaseCore {
+package su.nsk.iae.reflex.staticAnalysis.attributes;
+
+import org.antlr.v4.runtime.ParserRuleContext;
+import org.antlr.v4.runtime.misc.Pair;
+import su.nsk.iae.reflex.antlr.ReflexParser;
+
+import java.util.Vector;
+
+public class SwitchCaseCore implements IAttributed {
+    ParserRuleContext attributedContext;
+    ReflexParser.ProcessContext rootProcess;
+    ReflexParser.StateContext rootState;
+
+    Vector<SwitchCaseAttributes> branchAttributes;
+    SwitchCaseAttributes defaultBranchAttributes;
+
+    public SwitchCaseCore(ReflexParser.ProcessContext process, ReflexParser.StateContext state, ReflexParser.SwitchStatContext attributedContext){
+        rootProcess = process;
+        rootState = state;
+        this.attributedContext = attributedContext;
+    }
+
+    public void setAttributedContext(ParserRuleContext attributedContext) {
+        this.attributedContext = attributedContext;
+    }
+
+    public ReflexParser.ProcessContext getRootProcess() {
+        return rootProcess;
+    }
+
+    public void setRootProcess(ReflexParser.ProcessContext rootProcess) {
+        this.rootProcess = rootProcess;
+    }
+
+    public ReflexParser.StateContext getRootState() {
+        return rootState;
+    }
+
+    public void setRootState(ReflexParser.StateContext rootState) {
+        this.rootState = rootState;
+    }
+
+    public Vector<SwitchCaseAttributes> getBranchAttributes() {
+        return branchAttributes;
+    }
+
+    public void setBranchAttributes(Vector<SwitchCaseAttributes> branchAttributes) {
+        this.branchAttributes = branchAttributes;
+    }
+
+    public SwitchCaseAttributes getDefaultBranchAttributes() {
+        return defaultBranchAttributes;
+    }
+
+    public void addBranchAttributes(SwitchCaseAttributes attr){
+        this.branchAttributes.add(attr);
+    }
+
+    public void setDefaultBranchAttributes(SwitchCaseAttributes defaultBranchAttributes) {
+        this.defaultBranchAttributes = defaultBranchAttributes;
+    }
+
+    @Override
+    public ParserRuleContext getAttributedContext() {
+        return attributedContext;
+    }
+
+    @Override
+    public AttributedContextType getContextType() {
+        return AttributedContextType.SwitchCase;
+    }
 }
