src/main/java/su/nsk/iae/reflex/vcg/BranchPoint.java
@@ -2,9 +2,11 @@ package su.nsk.iae.reflex.vcg;
 
 import su.nsk.iae.reflex.antlr.ReflexParser;
 import su.nsk.iae.reflex.formulas.Formula;
+import su.nsk.iae.reflex.staticAnalysis.attributes.IAttributed;
 
 public class BranchPoint {
     Formula formula;
+    IAttributed attributed;
     ReflexParser.IfElseStContext ifCtx=null;
     ReflexParser.SwitchStContext switchCtx=null;
     ReflexParser.ProcessContext processCtx=null;
@@ -14,32 +16,36 @@ public class BranchPoint {
     String processName;
     String stateName;
 
-    public BranchPoint(Formula formula, ReflexParser.IfElseStContext ifCtx, Integer branch, Integer stateCount, String processName, String stateName) {
+    public BranchPoint(Formula formula, IAttributed attributed,ReflexParser.IfElseStContext ifCtx, Integer branch, Integer stateCount, String processName, String stateName) {
         this.formula = formula;
+        this.attributed = attributed;
         this.ifCtx = ifCtx;
         this.branch = branch;
         this.stateCount = stateCount;
         this.processName = processName;
         this.stateName = stateName;
     }
-    public BranchPoint(Formula formula, ReflexParser.SwitchStContext switchCtx, Integer branch, Integer stateCount, String processName, String stateName) {
+    public BranchPoint(Formula formula, IAttributed attributed,ReflexParser.SwitchStContext switchCtx, Integer branch, Integer stateCount, String processName, String stateName) {
         this.formula = formula;
+        this.attributed = attributed;
         this.switchCtx = switchCtx;
         this.branch = branch;
         this.stateCount = stateCount;
         this.processName = processName;
         this.stateName = stateName;
     }
-    public BranchPoint(Formula formula, ReflexParser.TimeoutFunctionContext timeoutCtx, Integer branch, Integer stateCount, String processName, String stateName) {
+    public BranchPoint(Formula formula, IAttributed attributed, ReflexParser.TimeoutFunctionContext timeoutCtx, Integer branch, Integer stateCount, String processName, String stateName) {
         this.formula = formula;
+        this.attributed = attributed;
         this.timeoutCtx = timeoutCtx;
         this.branch = branch;
         this.stateCount = stateCount;
         this.processName = processName;
         this.stateName = stateName;
     }
-    public BranchPoint(Formula formula, ReflexParser.ProcessContext processCtx, Integer branch, Integer stateCount, String processName, String stateName) {
+    public BranchPoint(Formula formula, IAttributed attributed, ReflexParser.ProcessContext processCtx, Integer branch, Integer stateCount, String processName, String stateName) {
         this.formula = formula;
+        this.attributed = attributed;
         this.processCtx = processCtx;
         this.branch = branch;
         this.stateCount = stateCount;
