src/main/java/su/nsk/iae/reflex/vcg/GenReturn.java
@@ -1,0 +1,12 @@
+package su.nsk.iae.reflex.vcg;
+
+public class GenReturn {
+    ReturnType returnType;
+
+    public GenReturn(ReturnType t){
+        returnType = t;
+    }
+    public ReturnType getReturnType() {
+        return returnType;
+    }
+}
