src/main/java/su/nsk/iae/reflex/vcg/ImpossibleVC.java
@@ -1,2 +1,0 @@
-package su.nsk.iae.reflex.vcg;public class ImpossibleVC {
-}
