src/main/java/su/nsk/iae/reflex/vcg/ReturnType.java
@@ -1,0 +1,5 @@
+package su.nsk.iae.reflex.vcg;
+
+public enum ReturnType {
+    Normal,ImpossibleVC
+}
