reflex_case_studies/Fridge/test/FridgeTheory.thy
@@ -1,5 +1,5 @@
 theory FridgeTheory
-imports Reflex
+imports ReflexPatterns
 begin
 
 fun ltime:: "state \<Rightarrow> process \<Rightarrow> nat" where 
@@ -25,14 +25,6 @@ lemma ltime_mult:
 "ltime s p mod 100 = 0"
   by (induction s) (auto)
 
-lemma ltime_mod:
-assumes "ltime s0 p < a*100"
-shows "ltime s0 p ≤ (a*100-100)"
-proof -
-have"(ltime s0 p) mod 100 = 0" by (induction s0) (auto)
-thus ?thesis using assms by (induction a) (auto)
-qed
-
 lemma ltime_div_less:
 assumes "(ltime s0 p div 100)≤ a"
 shows "(ltime s0 p -100) div 100 < a ∨ ltime s0 p = 0"
@@ -46,5 +38,15 @@ lemma ltime_le_toEnvNum:
   apply(induction s)
          apply(auto)
   done
+lemma toEnvNum_getPstate:
+"toEnvNum s s' < ltime s' p div 100 \<Rightarrow> getPstate s p = getPstate s' p"
+  apply (induction s' arbitrary:s)
+  apply auto
+  apply (metis Suc_eq_plus1 getPstate.simps(2) not_less_eq)
+  using getPstate.simps apply presburger+
+done
 
+lemma inter_toEnvNum_getPstate:
+"toEnvNum s s' < ltime s' p div 100 ∧ substate s s'' ∧ substate s'' s'\<Rightarrow> toEnvNum s'' s' < ltime s' p div 100"
+  using toEnvNum3 by fastforce
 end
