reflex_case_studies/Fridge/test/Fridge_VC72.thy
@@ -1,0 +1,30 @@
+theory Fridge_VC72
+imports FridgeTheory
+begin
+
+lemma
+ assumes base_inv:"(inv st0)"
+ and st1:"(st1=(setVarBool st0 ''inp_3'' inp_3))"
+ and st2:"(st2=(setVarBool st1 ''inp_2'' inp_2))"
+ and st3:"(st3=(setVarBool st2 ''inp_1'' inp_1))"
+ and st4:"(st4=(setVarBool st3 ''inp_5'' inp_5))"
+ and st5:"(st5=(setVarBool st4 ''inp_4'' inp_4))"
+ and st5_Init_state:"(getPstate st5 ''Init'')=''begin''"
+ and st6:"(st6=(setPstate st5 ''FridgrDoorController'' ''closed''))"
+ and st7:"(st7=(setPstate st6 ''FridgeCompressorController'' ''checkTemp''))"
+ and st8:"(st8=(setPstate st7 ''FreezerCompressorController'' ''checkTemp''))"
+ and st9:"(st9=(setPstate st8 ''Init'' ''''stop''''))"
+ and st9_FridgrDoorController_state:"(getPstate st9 ''FridgrDoorController'')=''open''"
+ and st9_open_timeout:"30000\<le>(ltime st9 ''FridgrDoorController'')"
+ and st10:"(st10=(setVarBool st9 ''out_4'' True))"
+ and st11:"(st11=(setPstate st10 ''FridgrDoorController'' ''longOpen''))"
+ and st11_FridgeCompressorController_state:"(getPstate st11 ''FridgeCompressorController'')=''checkTemp''"
+ and st11_if19:"(getVarBool st11 ''inp_2'')=False"
+ and st11_FreezerCompressorController_state:"(getPstate st11 ''FreezerCompressorController'')=''checkTemp''"
+ and st11_if21:"(getVarBool st11 ''inp_4'')=True"
+ and st12:"(st12=(setVarBool st11 ''out_2'' True))"
+ and st13:"(st13=(toEnv st12))"
+ and st_final:"(st_final=st13)"
+shows "(inv st_final)"
+
+end
